untyped4 - split to arg + upvar

src/Untyped4.v
@@ -5,17 +5,12 @@ Require Import Metadata.
 Require Import Semantics.
 Require Import HighestValues.
 
-(* TODO:
- - directly run_cont from SConstrDone/SCloseDone
- - unflag values
- - convert to functional continuations
- *)
-
 
 
 Inductive expr :=
 | Value (v : value)
-| Var (idx : nat)
+| Arg
+| UpVar (idx : nat)
 | App (f : expr) (a : expr)
 | MkConstr (ctor : constr_name) (args : list expr)
 | MkClose (fname : nat) (free : list expr)
@@ -41,69 +36,6 @@ Inductive state :=
 | Run (e : expr) (l : list value) (k : cont)
 | Stop (v : value)
 .
-
-
-Definition weaken_value :=
-    let fix go v :=
-        let fix go_list vs :=
-            match vs with
-            | [] => []
-            | v :: vs => go v :: go_list vs
-            end in
-        match v with
-        | Constr ctor args => Constr ctor (go_list args)
-        | Close fname free => Close (S fname) (go_list free)
-        end in go.
-
-Definition weaken_value_list :=
-    let go := weaken_value in
-    let fix go_list es :=
-        match es with
-        | [] => []
-        | e :: es => go e :: go_list es
-        end in go_list.
-
-Definition weaken_expr :=
-    let fix go e :=
-        let fix go_list es :=
-            match es with
-            | [] => []
-            | e :: es => go e :: go_list es
-            end in
-        match e with
-        | Value v => Value (weaken_value v)
-        | Var idx => Var idx
-        | App f a => App (go f) (go a)
-        | MkConstr ctor args => MkConstr ctor (go_list args)
-        | MkClose fname free => MkClose (S fname) (go_list free)
-        | Elim ty cases target => Elim ty (go_list cases) (go target)
-        end in go.
-
-Definition weaken_expr_list :=
-    let go := weaken_expr in
-    let fix go_list es :=
-        match es with
-        | [] => []
-        | e :: es => go e :: go_list es
-        end in go_list.
-
-Fixpoint get_weaken g n :=
-    match n with
-    | 0 =>
-            match g with
-            | [] => None
-            | e :: _ => Some (weaken_expr e)
-            end
-    | S n' =>
-            match g with
-            | [] => None
-            | _ :: g' =>
-                    match get_weaken g' n' with
-                    | Some e => Some (weaken_expr e)
-                    | None => None
-                    end
-            end
-    end.
 
 
 (* helper function for proceeding into a continuation *)
@@ -139,25 +71,20 @@ Fixpoint unroll_elim' (case : expr)
 Definition unroll_elim case ctor args mk_rec :=
     unroll_elim' case ctor args mk_rec 0.
 
-Definition run_elim (ty : type_name) (cases : list expr) (target : value) :=
-    match target with
-    | Constr ctor args =>
-            match nth_error cases (constructor_index ctor) with
-            | Some case => Some (unroll_elim case ctor args (Elim ty cases))
-            | None => None
-            end
-    | _ => None
-    end.
-
 (* the actual step relation *)
 Inductive sstep (g : list expr) : state -> state -> Prop :=
 | SValue : forall v (l : list value) (k : cont),
         sstep g (Run (Value v) l k)
                 (run_cont k v)
 
-| SVar : forall idx (l : list value) (k : cont) v,
-        nth_error l idx = Some v ->
-        sstep g (Run (Var idx) l k)
+| SArg : forall (l : list value) (k : cont) v,
+        nth_error l 0 = Some v ->
+        sstep g (Run (Arg) l k)
+                (Run (Value v) l k)
+
+| SUpVar : forall idx (l : list value) (k : cont) v,
+        nth_error l (S idx) = Some v ->
+        sstep g (Run (UpVar idx) l k)
                 (Run (Value v) l k)
 
 | SAppL : forall (e1 : expr) (e2 : expr) l k,
@@ -172,7 +99,7 @@ Inductive sstep (g : list expr) : state -> state -> Prop :=
                 (Run e2 l (KAppR e1 l k))
 
 | SMakeCall : forall fname free arg l k body,
-        get_weaken g fname = Some body ->
+        nth_error g fname = Some body ->
         sstep g (Run (App (Value (Close fname free)) (Value arg)) l k)
                 (Run body (arg :: free) k)
 
@@ -228,11 +155,13 @@ Inductive sstep (g : list expr) : state -> state -> Prop :=
             (cases : list expr)
             (ctor : constr_name)
             (args : list value)
+            (case : expr)
             (result : expr)
             l k,
         is_ctor_for_type ty ctor ->
         constructor_arg_n ctor = length args ->
-        run_elim ty cases (Constr ctor args) = Some result ->
+        nth_error cases (constructor_index ctor) = Some case ->
+        unroll_elim case ctor args (Elim ty cases) = result ->
         sstep g (Run (Elim ty cases (Value (Constr ctor args))) l k)
                 (Run result l k)
 .
